reworking into total functions

IndexFunctions.v
@@ -19,10 +19,9 @@ Require Import MathClasses.orders.orders.
 Global Open Scope nat_scope.
 
 (* Vector index mapping functon which maps between two sets of natrual
-     numers. Mapping is partial and it returns None if there is no correspondance
-     between a number in source set and target set. *)
+     numers. *)
 Definition index_map_spec (domain range: nat) :=
-  forall n : nat, n < domain -> {v : option nat | forall n' : nat, v ≡ Some n' -> n' < range}.
+  forall n : nat, n < domain -> {v : nat | v < range}.
 
 (* Returns upper domain bound for given `index_map_spec` *)
 Definition index_map_dom {d r:nat} (s: index_map_spec d r) := d.
@@ -30,98 +29,83 @@ Definition index_map_dom {d r:nat} (s: index_map_spec d r) := d.
 (* Returns upper rang bound for given `index_map_spec` *)
 Definition index_map_range {d r:nat} (s: index_map_spec d r) := r.
 
-Section TotalIndexMap.
-
-  (* Vector index mapping functon which maps between two sets of natrual
-     numers. *)
-  Definition total_index_map_spec (domain range: nat) :=
-    forall n : nat, n < domain -> {v : nat | v < range}.
+Section Primitive_Functions.
   
-  (* Returns upper domain bound for given `total_index_map_spec` *)
-  Definition total_index_map_dom {d r:nat} (s: total_index_map_spec d r) := d.
+  Program Definition identity_index_map
+          {domain range: nat}
+          {drdep: domain ≡ range}:
+    index_map_spec domain range
+    :=
+      fun i i_dim => i.
   
-  (* Returns upper rang bound for given `total_index_map_spec` *)
-  Definition total_index_map_range {d r:nat} (s: total_index_map_spec d r) := r.
-
-  Section Primitive_Functions.
-    
-    Program Definition identity_index_map
-            {domain range: nat}
-            {drdep: domain ≡ range}:
-      total_index_map_spec domain range
-      :=
-        fun i i_dim => i.
-    
-    Program Definition constant_index_map
-            {range: nat}
-            (j: nat)
-            {jdep: j<range}:
-      total_index_map_spec 1%nat range
-      :=
-        fun _ _ => j.
-    
-    Program Definition add_index_map
-            {domain range: nat}
-            (k: nat)
-            {kdep: k+domain <= range}:
-      total_index_map_spec domain range
-      :=
-        fun i i_dim => i+k.
-    Next Obligation.
-      lia.
-    Defined.
-
-  End Primitive_Functions.
-
-  Section Function_Operators.
-    
-    Definition total_index_map_compose
-               {i o t: nat}
-               (g: total_index_map_spec t o)
-               (f: total_index_map_spec i t) :
-      total_index_map_spec i o
-      := fun x xdom_bound =>
-           (* manual uncurry *)
-           let (fv, fv_dom_bound) := f x xdom_bound in
-           g fv fv_dom_bound.
-
-    Program Definition total_index_map_tensor_product
-               {m n M N: nat}
-               {nz: 0 ≢ n}
-               (f: total_index_map_spec m M)
-               (g: total_index_map_spec n N):
-      total_index_map_spec (m*n) (M*N)
-      := fun i _ =>
-           let pn := pred n in
-           let ab := divmod i pn 0 pn in
-           N * (f (fst ab) _) + (g (pn - (snd ab)) _).
-    Next Obligation.
-      destruct n.
-      congruence. clear nz.
-      simpl.
-      generalize (divmod_spec i n 0 n). 
-      destruct divmod as (q,u).
-      simpl.
-      nia.
-    Defined.
-    Next Obligation.
-      destruct n.
-      congruence. clear nz.
-      lia.
-    Defined.
-    Next Obligation.
-      generalize (f (fst (divmod i (pred n) 0 (pred n)))
-                    (total_index_map_tensor_product_obligation_1 m n M N nz f g i H)) as fg.
-      generalize (g (pred n - snd (divmod i (pred n) 0 (pred n)))
-                    (total_index_map_tensor_product_obligation_2 m n M N nz f g i H)) as gg.
-      intros.
-      destruct gg as [gv ga].
-      destruct fg as [fv fa].
-      simpl.
-      nia.
-    Defined.
-    
-  End Function_Operators.
+  Program Definition constant_index_map
+          {range: nat}
+          (j: nat)
+          {jdep: j<range}:
+    index_map_spec 1%nat range
+    :=
+      fun _ _ => j.
   
+  Program Definition add_index_map
+          {domain range: nat}
+          (k: nat)
+          {kdep: k+domain <= range}:
+    index_map_spec domain range
+    :=
+      fun i i_dim => i+k.
+  Next Obligation.
+    lia.
+  Defined.
+
+End Primitive_Functions.
+
+Section Function_Operators.
   
-End TotalIndexMap.
+  Definition index_map_compose
+             {i o t: nat}
+             (g: index_map_spec t o)
+             (f: index_map_spec i t) :
+    index_map_spec i o
+    := fun x xdom_bound =>
+         (* manual uncurry *)
+         let (fv, fv_dom_bound) := f x xdom_bound in
+         g fv fv_dom_bound.
+
+  Program Definition index_map_tensor_product
+          {m n M N: nat}
+          {nz: 0 ≢ n}
+          (f: index_map_spec m M)
+          (g: index_map_spec n N):
+    index_map_spec (m*n) (M*N)
+    := fun i _ =>
+         let pn := pred n in
+         let ab := divmod i pn 0 pn in
+         N * (f (fst ab) _) + (g (pn - (snd ab)) _).
+  Next Obligation.
+    destruct n.
+    congruence. clear nz.
+    simpl.
+    generalize (divmod_spec i n 0 n). 
+    destruct divmod as (q,u).
+    simpl.
+    nia.
+  Defined.
+  Next Obligation.
+    destruct n.
+    congruence. clear nz.
+    lia.
+  Defined.
+  Next Obligation.
+    generalize (f (fst (divmod i (pred n) 0 (pred n)))
+                  (index_map_tensor_product_obligation_1 m n M N nz f g i H)) as fg.
+    generalize (g (pred n - snd (divmod i (pred n) 0 (pred n)))
+                  (index_map_tensor_product_obligation_2 m n M N nz f g i H)) as gg.
+    intros.
+    destruct gg as [gv ga].
+    destruct fg as [fv fa].
+    simpl.
+    nia.
+  Defined.
+  
+End Function_Operators.
+
